src/Std/Tactic/BVDecide/Bitblast/BVExpr/Circuit/Lemmas.lean
@@ -20,9 +20,85 @@ open Std.Sat.AIG
 
 namespace BVLogicalExpr
 
-namespace bitblast
+namespace Cache
 
-mutual
+abbrev Inv (assign : BVExpr.Assignment) (aig : AIG BVBit) (cache : Cache aig) : Prop :=
+  ∀ expr (h : expr ∈ cache.map),
+    ⟦aig, ⟨(cache.map[expr]'h).1, (cache.map[expr]'h).2, cache.hbound ..⟩, assign.toAIGAssignment⟧
+      =
+    expr.eval assign
+
+theorem Inv_empty (aig : AIG BVBit) : Inv assign aig Cache.empty := by
+  intro k hk
+  simp [Cache.empty] at hk
+
+theorem Inv_cast (cache : Cache aig1) (hpref : IsPrefix aig1.decls aig2.decls)
+    (hinv : Inv assign aig1 cache):
+    Inv assign aig2 (cache.cast hpref.size_le) := by
+  unfold Cache.cast
+  intro expr hexpr
+  specialize hinv expr hexpr
+  rw [← hinv]
+  apply denote.eq_of_isPrefix (entry := ⟨aig1, _, _, _⟩)
+  exact hpref
+
+theorem Inv_insert (cache : Cache aig) (expr : BVLogicalExpr) (ref : AIG.Ref aig)
+    (hinv : Inv assign aig cache)
+    (href : ⟦aig, ref, assign.toAIGAssignment⟧ = expr.eval assign) :
+    Inv assign aig (cache.insert expr ref) := by
+  intro k hk
+  by_cases heq : expr = k
+  · subst heq
+    have : ((cache.insert expr ref).map[expr]'hk) = (ref.gate, ref.invert) := by
+      unfold Cache.insert
+      apply Std.HashMap.getElem_insert_self
+    rw [← href]
+    congr 3
+    all_goals
+      rw [this]
+  · have hmem : k ∈ cache.map := by
+      unfold Cache.insert at hk
+      apply Std.HashMap.mem_of_mem_insert
+      · exact hk
+      · simp [heq]
+    have : ((cache.insert expr ref).map[k]'hk) = cache.map[k]'hmem := by
+      unfold Cache.insert
+      rw [Std.HashMap.getElem_insert]
+      simp [heq]
+    rw [← hinv]
+    congr 3
+    all_goals
+      rw [this]
+
+theorem get?_eq_some_iff (cache : Cache aig) (expr : BVLogicalExpr) :
+    cache.get? expr = some ref ↔ cache.map[expr]? = some (ref.gate, ref.invert) := by
+  cases ref
+  unfold Cache.get?
+  split
+  · next ref heq => cases ref; simp [heq]
+  · next heq => simp [heq]
+
+theorem denote_eq_eval_of_get?_eq_some_of_Inv (cache : Cache aig) (expr : BVLogicalExpr)
+    (ref : AIG.Ref aig) (hsome : cache.get? expr = some ref) (hinv : Inv assign aig cache) :
+    ⟦aig,  ref, assign.toAIGAssignment⟧ = expr.eval assign := by
+  rw [get?_eq_some_iff] at hsome
+  have hmem : expr ∈ cache.map := by
+    rw [Std.HashMap.mem_iff_contains, Std.HashMap.contains_eq_isSome_getElem?]
+    simp [hsome]
+  have href : cache.map[expr]'hmem = (ref.gate, ref.invert) := by
+    rw [Std.HashMap.getElem?_eq_some_getElem (h' := hmem)] at hsome
+    simp only [Option.some.injEq] at hsome
+    rw [hsome]
+  specialize hinv expr hmem
+  rw [← hinv]
+  cases ref
+  congr 3
+  all_goals
+    rw [href]
+
+end Cache
+
+namespace bitblast
 
 theorem go_Inv_of_Inv (expr : BVLogicalExpr) (aig : AIG BVBit) (assign : BVExpr.Assignment)
     (bvCache : BVExpr.Cache aig) (logCache : Cache aig) (hinv1 : BVExpr.Cache.Inv assign aig bvCache) :
@@ -62,6 +138,8 @@ theorem go_Inv_of_Inv (expr : BVLogicalExpr) (aig : AIG BVBit) (assign : BVExpr.
       apply lih
       apply dih
       exact hinv -/
+
+mutual
 
 theorem go_eval_eq_eval (expr : BVLogicalExpr) (aig : AIG BVBit) (assign : BVExpr.Assignment)
     (bvCache : BVExpr.Cache aig) (hinv : BVExpr.Cache.Inv assign aig bvCache)
